\documentclass[11]{article}
\usepackage{amsmath}
\usepackage{csquotes}
\usepackage{amssymb}
\usepackage{hyperref}
\newlength\tindent
\setlength{\tindent}{\parindent}
\setlength{\parindent}{0pt}
\renewcommand{\indent}{\hspace*{\tindent}}

\title{\sc{I Dislike Differential Equations}}
\author{\sc{Rahul}}
\date{26 April, 2025}
\begin{document}
\maketitle
i was doing some random DE. It simplified to this:

$$\frac{x dy - y dx}{x^2 + y^2}$$

Now instead of homogenizing it or whatever like a normal person, i saw that the denominator was $|z|^2$ where $z = x+iy$. See where i'm going with this?

$$z = x + iy$$
$$dz = dx + i dy$$
$$\bar{z} \ dz = (x \ dx + y \ dy) + i (x \ dy - y \ dx)$$
$$\frac{\bar{z} \ dz}{z \bar{z}} = \frac{(x \ dx + y \ dy) + i (x \ dy - y \ dx)}{x^2 + y^2}$$
$$ d(\ln z) =  \frac{(x \ dx + y \ dy)}{x^2 + y^2} + i \frac{(x \ dy - y \ dx)}{x^2 + y^2}$$

Now using $z = r e^{i \theta}$, we get $\ln z = \ln r + i \theta$. Equating real and imaginary components:

$$\boxed{ \frac{(x \ dx + y \ dy)}{x^2 + y^2} = d(\ln \sqrt{x^2+y^2})}$$

$$\boxed{\frac{(x \ dy - y \ dx)}{x^2 + y^2} = d\left(\tan^{-1} \frac{y}{x}\right)}$$

(typing this i realise this is just polar coordinates. but still)

\end{document}